Fix allocator to promise strict inequality
This requires a technical condition that max be > 0, which is
incorporated as a new opaque Valid() predicate. I was hoping we could
get away without one but this does make it a bit easier to use.

src/dafny_go/jrnl/alloc.go
@@ -7,6 +7,9 @@ type Allocator struct {
 }
 
 func NewAllocator(max uint64) *Allocator {
+	if max == 0 {
+		panic("invalid max, must be at least 0")
+	}
 	num_bytes := max / 8
 	a := alloc.MkAlloc(make([]byte, num_bytes))
 	return &Allocator{alloc: *a}
